experiments/coq/Tactics.v
@@ -1,13 +1,33 @@
-Ltac destructo :=
+Ltac destruct_b :=
   repeat
     match goal with
     | [ H : context [ match ?X with _ => _ end ] |- _ ] =>
       match type of X with
-      | option _ => destruct X
+      | prod _ _ => destruct X eqn:?
+      | sum  _ _ => destruct X eqn:?
+      | option _ => destruct X eqn:?
+      | list _   => destruct X eqn:?
+      end
+    | [ H : context [ let _ := ?X in _ ] |- _ ] =>
+      match type of X with
+      | prod _ _ => destruct X eqn:?
+      | sum  _ _ => destruct X eqn:?
+      | option _ => destruct X eqn:?
+      | list _   => destruct X eqn:?
       end
     | [ |- context [ match ?X with _ => _ end ] ] =>
       match type of X with
-      | option _ => destruct X
+      | prod _ _ => destruct X eqn:?
+      | sum  _ _ => destruct X eqn:?
+      | option _ => destruct X eqn:?
+      | list   _ => destruct X eqn:?
+      end
+    | [ |- context [ let _ := ?X in _ ] ] =>
+      match type of X with
+      | prod _ _ => destruct X eqn:?
+      | sum  _ _ => destruct X eqn:?
+      | option _ => destruct X eqn:?
+      | list   _ => destruct X eqn:?
       end
     end.
 
@@ -17,6 +37,9 @@ Ltac destruct_if :=
     | [ H : context [ if ?X then _ else _ ] |- _ ] => destruct X
     | [ |- context [ if ?X then _ else _ ] ] => destruct X
     end.
+
+Ltac destructo :=
+  destruct_b; destruct_if; subst.
 
 Ltac invert H :=
   inversion H; subst; clear H.
